<?xml version='1.0' encoding='UTF-8'?>
<rdf:RDF xmlns:rdf="http://www.w3.org/1999/02/22-rdf-syntax-ns#" xmlns:rdfs="http://www.w3.org/2000/01/rdf-schema#" xmlns:owl="http://www.w3.org/2002/07/owl#" xmlns:xsd="http://www.w3.org/2001/XMLSchema#" xmlns:dc="http://purl.org/dc/elements/1.1/" xmlns:skos="http://www.w3.org/2004/02/skos/core#" xmlns:schema="http://schema.org/" xmlns:prov="http://www.w3.org/ns/prov#" xmlns:merge="http://example.org/merged-ontology/" xml:base="http://example.org/merged-ontology/1.0"><owl:Ontology rdf:about="http://example.org/merged-ontology/1.0"><dc:title xml:lang="en">Merged Ontology</dc:title><dc:description xml:lang="en">A new ontology that selectively imports classes and properties from PPEO and SOSA, preserving original IRIs and all OWL axioms.</dc:description><rdfs:seeAlso rdf:resource="http://purl.org/ppeo/PPEO.owl"/><rdfs:seeAlso rdf:resource="http://www.w3.org/ns/sosa/"/></owl:Ontology><owl:Class rdf:about="http://purl.org/ppeo/PPEO.owl#data_file">
        <rdfs:subClassOf>
            <owl:Restriction>
                <owl:onProperty rdf:resource="http://purl.org/ppeo/PPEO.owl#hasDescription"/>
                <owl:qualifiedCardinality rdf:datatype="http://www.w3.org/2001/XMLSchema#nonNegativeInteger">1</owl:qualifiedCardinality>
                <owl:onDataRange rdf:resource="http://www.w3.org/2001/XMLSchema#string"/>
            </owl:Restriction>
        </rdfs:subClassOf>
        <rdfs:subClassOf>
            <owl:Restriction>
                <owl:onProperty rdf:resource="http://purl.org/ppeo/PPEO.owl#hasDigitalLocation"/>
                <owl:qualifiedCardinality rdf:datatype="http://www.w3.org/2001/XMLSchema#nonNegativeInteger">1</owl:qualifiedCardinality>
                <owl:onDataRange>
                    <rdfs:Datatype>
                        <owl:unionOf rdf:parseType="Collection">
                            <rdf:Description rdf:about="http://www.w3.org/2001/XMLSchema#anyURI"/>
                            <rdf:Description rdf:about="http://www.w3.org/2001/XMLSchema#string"/>
                        </owl:unionOf>
                    </rdfs:Datatype>
                </owl:onDataRange>
            </owl:Restriction>
        </rdfs:subClassOf>
        <rdfs:subClassOf>
            <owl:Restriction>
                <owl:onProperty rdf:resource="http://purl.org/ppeo/PPEO.owl#hasVersion"/>
                <owl:qualifiedCardinality rdf:datatype="http://www.w3.org/2001/XMLSchema#nonNegativeInteger">1</owl:qualifiedCardinality>
                <owl:onDataRange rdf:resource="http://www.w3.org/2001/XMLSchema#string"/>
            </owl:Restriction>
        </rdfs:subClassOf>
        <rdfs:comment xml:lang="en">A description of and link to a file or data stream holding some or all of the data described by the MIAPPE submission.</rdfs:comment>
        <rdfs:label xml:lang="en">data file</rdfs:label>
    <merge:sourcedFrom rdf:datatype="http://www.w3.org/2001/XMLSchema#anyURI">http://purl.org/ppeo/PPEO.owl</merge:sourcedFrom><merge:sourceOntology>ppeo</merge:sourceOntology></owl:Class>
    


    <owl:ObjectProperty rdf:about="http://purl.org/ppeo/PPEO.owl#hasObservation">
        <rdfs:domain rdf:resource="http://purl.org/ppeo/PPEO.owl#data_file"/>
        <rdfs:range rdf:resource="http://purl.org/ppeo/PPEO.owl#observation"/>
        <rdfs:label xml:lang="en">has observation</rdfs:label>
    <merge:sourcedFrom rdf:datatype="http://www.w3.org/2001/XMLSchema#anyURI">http://purl.org/ppeo/PPEO.owl</merge:sourcedFrom><merge:sourceOntology>ppeo</merge:sourceOntology></owl:ObjectProperty>
    


    <owl:Class rdf:about="http://purl.org/ppeo/PPEO.owl#observation">
        <rdfs:subClassOf>
            <owl:Restriction>
                <owl:onProperty rdf:resource="http://purl.org/ppeo/PPEO.owl#hasObservedSubject"/>
                <owl:qualifiedCardinality rdf:datatype="http://www.w3.org/2001/XMLSchema#nonNegativeInteger">1</owl:qualifiedCardinality>
                <owl:onClass>
                    <owl:Class>
                        <owl:unionOf rdf:parseType="Collection">
                            <rdf:Description rdf:about="http://purl.org/ppeo/PPEO.owl#observation_unit"/>
                            <rdf:Description rdf:about="http://purl.org/ppeo/PPEO.owl#sample"/>
                        </owl:unionOf>
                    </owl:Class>
                </owl:onClass>
            </owl:Restriction>
        </rdfs:subClassOf>
        <rdfs:subClassOf>
            <owl:Restriction>
                <owl:onProperty rdf:resource="http://purl.org/ppeo/PPEO.owl#hasVariable"/>
                <owl:qualifiedCardinality rdf:datatype="http://www.w3.org/2001/XMLSchema#nonNegativeInteger">1</owl:qualifiedCardinality>
                <owl:onClass rdf:resource="http://purl.org/ppeo/PPEO.owl#observed_variable"/>
            </owl:Restriction>
        </rdfs:subClassOf>
        <rdfs:subClassOf>
            <owl:Restriction>
                <owl:onProperty rdf:resource="http://purl.org/ppeo/PPEO.owl#hasValue"/>
                <owl:allValuesFrom>
                    <rdfs:Datatype>
                        <owl:unionOf rdf:parseType="Collection">
                            <rdf:Description rdf:about="http://www.w3.org/2001/XMLSchema#float"/>
                            <rdf:Description rdf:about="http://www.w3.org/2001/XMLSchema#int"/>
                            <rdf:Description rdf:about="http://www.w3.org/2001/XMLSchema#string"/>
                        </owl:unionOf>
                    </rdfs:Datatype>
                </owl:allValuesFrom>
            </owl:Restriction>
        </rdfs:subClassOf>
        <rdfs:label xml:lang="en">observation</rdfs:label>
    <merge:sourcedFrom rdf:datatype="http://www.w3.org/2001/XMLSchema#anyURI">http://purl.org/ppeo/PPEO.owl</merge:sourcedFrom><merge:sourceOntology>ppeo</merge:sourceOntology></owl:Class>
    


    <owl:Class rdf:about="http://www.w3.org/ns/sosa/Observation">
		<rdfs:label xml:lang="en">Observation</rdfs:label>
		<rdfs:comment xml:lang="en">Act of carrying out an (Observation) Procedure to estimate or calculate a value of a property of a FeatureOfInterest. Links to a Sensor to describe what made the Observation and how; links to an ObservableProperty to describe what the result is an estimate of, and to a FeatureOfInterest to detail what that property was associated with.</rdfs:comment>
		<rdfs:isDefinedBy rdf:resource="http://www.w3.org/ns/sosa/"/>
		<skos:definition xml:lang="en">Act of carrying out an (Observation) Procedure to estimate or calculate a value of a property of a FeatureOfInterest. Links to a Sensor to describe what made the Observation and how; links to an ObservableProperty to describe what the result is an estimate of, and to a FeatureOfInterest to detail what that property was associated with.</skos:definition>
		<skos:example xml:lang="en">The activity of estimating the intensity of an Earthquake using the Mercalli intensity scale is an Observation as is measuring the moment magnitude, i.e., the energy released by said earthquake.</skos:example>
	<merge:sourcedFrom rdf:datatype="http://www.w3.org/2001/XMLSchema#anyURI">http://www.w3.org/ns/sosa/</merge:sourcedFrom><merge:sourceOntology>sosa</merge:sourceOntology></owl:Class>
	
	<owl:Class rdf:about="http://www.w3.org/ns/sosa/Sensor">
		<rdfs:label xml:lang="en">Sensor</rdfs:label>
		<rdfs:comment xml:lang="en">Device, agent (including humans), or software (simulation) involved in, or implementing, a Procedure. Sensors respond to a stimulus, e.g., a change in the environment, or input data composed from the results of prior Observations, and generate a Result. Sensors can be hosted by Platforms.</rdfs:comment>
		<rdfs:isDefinedBy rdf:resource="http://www.w3.org/ns/sosa/"/>
		<skos:definition xml:lang="en">Device, agent (including humans), or software (simulation) involved in, or implementing, a Procedure. Sensors respond to a stimulus, e.g., a change in the environment, or input data composed from the results of prior Observations, and generate a Result. Sensors can be hosted by Platforms.</skos:definition>
		<skos:example xml:lang="en">Accelerometers, gyroscopes, barometers, magnetometers, and so forth are Sensors that are typically mounted on a modern smart phone (which acts as Platform). Other examples of sensors include the human eyes.</skos:example>
	<merge:sourcedFrom rdf:datatype="http://www.w3.org/2001/XMLSchema#anyURI">http://www.w3.org/ns/sosa/</merge:sourcedFrom><merge:sourceOntology>sosa</merge:sourceOntology></owl:Class>
	
	<owl:ObjectProperty rdf:about="http://www.w3.org/ns/sosa/madeBySensor">
		<rdfs:label xml:lang="en">made by sensor</rdfs:label>
		<rdfs:comment xml:lang="en">Relation between an Observation and the Sensor which made the Observation.</rdfs:comment>
		<schema:domainIncludes rdf:resource="http://www.w3.org/ns/sosa/Observation"/>
		<schema:rangeIncludes rdf:resource="http://www.w3.org/ns/sosa/Sensor"/>
		<rdfs:isDefinedBy rdf:resource="http://www.w3.org/ns/sosa/"/>
		<owl:inverseOf rdf:resource="http://www.w3.org/ns/sosa/madeObservation"/>
		<skos:definition xml:lang="en">Relation between an Observation and the Sensor which made the Observation.</skos:definition>
	<merge:sourcedFrom rdf:datatype="http://www.w3.org/2001/XMLSchema#anyURI">http://www.w3.org/ns/sosa/</merge:sourcedFrom><merge:sourceOntology>sosa</merge:sourceOntology></owl:ObjectProperty>
	
	<owl:DatatypeProperty rdf:about="http://purl.org/ppeo/PPEO.owl#hasDescription"><rdfs:label xml:lang="en">has description</rdfs:label>
    <merge:sourcedFrom rdf:datatype="http://www.w3.org/2001/XMLSchema#anyURI">http://purl.org/ppeo/PPEO.owl</merge:sourcedFrom><merge:sourceOntology>ppeo</merge:sourceOntology></owl:DatatypeProperty><owl:DatatypeProperty rdf:about="http://purl.org/ppeo/PPEO.owl#hasDigitalLocation"><rdfs:comment xml:lang="en">The location of the file in the form of a URI or,  if the file is contained within a local MIAPPE submission (e.g. ISA-Tab), a path or file name.</rdfs:comment>
        <rdfs:label xml:lang="en">has digital location</rdfs:label>
    <merge:sourcedFrom rdf:datatype="http://www.w3.org/2001/XMLSchema#anyURI">http://purl.org/ppeo/PPEO.owl</merge:sourcedFrom><merge:sourceOntology>ppeo</merge:sourceOntology></owl:DatatypeProperty><owl:ObjectProperty rdf:about="http://purl.org/ppeo/PPEO.owl#hasObservedSubject"><rdfs:label xml:lang="en">has observed subject</rdfs:label>
    <merge:sourcedFrom rdf:datatype="http://www.w3.org/2001/XMLSchema#anyURI">http://purl.org/ppeo/PPEO.owl</merge:sourcedFrom><merge:sourceOntology>ppeo</merge:sourceOntology></owl:ObjectProperty><owl:DatatypeProperty rdf:about="http://purl.org/ppeo/PPEO.owl#hasValue"><rdfs:label xml:lang="en">has value</rdfs:label>
    <merge:sourcedFrom rdf:datatype="http://www.w3.org/2001/XMLSchema#anyURI">http://purl.org/ppeo/PPEO.owl</merge:sourcedFrom><merge:sourceOntology>ppeo</merge:sourceOntology></owl:DatatypeProperty><owl:ObjectProperty rdf:about="http://purl.org/ppeo/PPEO.owl#hasVariable"><rdfs:label xml:lang="en">has variable</rdfs:label>
    <merge:sourcedFrom rdf:datatype="http://www.w3.org/2001/XMLSchema#anyURI">http://purl.org/ppeo/PPEO.owl</merge:sourcedFrom><merge:sourceOntology>ppeo</merge:sourceOntology></owl:ObjectProperty><owl:DatatypeProperty rdf:about="http://purl.org/ppeo/PPEO.owl#hasVersion"><rdfs:label xml:lang="en">has version</rdfs:label>
    <merge:sourcedFrom rdf:datatype="http://www.w3.org/2001/XMLSchema#anyURI">http://purl.org/ppeo/PPEO.owl</merge:sourcedFrom><merge:sourceOntology>ppeo</merge:sourceOntology></owl:DatatypeProperty><owl:ObjectProperty rdf:about="http://www.w3.org/ns/sosa/madeObservation"><rdfs:label xml:lang="en">made observation</rdfs:label>
		<rdfs:comment xml:lang="en">Relation between a Sensor and an Observation made by the Sensor.</rdfs:comment>
		<rdfs:isDefinedBy rdf:resource="http://www.w3.org/ns/sosa/"/>
		<skos:definition xml:lang="en">Relation between a Sensor and an Observation made by the Sensor.</skos:definition>
	<merge:sourcedFrom rdf:datatype="http://www.w3.org/2001/XMLSchema#anyURI">http://www.w3.org/ns/sosa/</merge:sourcedFrom><merge:sourceOntology>sosa</merge:sourceOntology></owl:ObjectProperty><owl:Class rdf:about="http://purl.org/ppeo/PPEO.owl#observation_unit"><rdfs:label xml:lang="en">observation unit</rdfs:label>
    <merge:sourcedFrom rdf:datatype="http://www.w3.org/2001/XMLSchema#anyURI">http://purl.org/ppeo/PPEO.owl</merge:sourcedFrom><merge:sourceOntology>ppeo</merge:sourceOntology></owl:Class><owl:Class rdf:about="http://purl.org/ppeo/PPEO.owl#observed_variable"><rdfs:label xml:lang="en">observed variable</rdfs:label>
    <merge:sourcedFrom rdf:datatype="http://www.w3.org/2001/XMLSchema#anyURI">http://purl.org/ppeo/PPEO.owl</merge:sourcedFrom><merge:sourceOntology>ppeo</merge:sourceOntology></owl:Class><owl:Class rdf:about="http://purl.org/ppeo/PPEO.owl#sample"><rdfs:label xml:lang="en">sample</rdfs:label>
    <merge:sourcedFrom rdf:datatype="http://www.w3.org/2001/XMLSchema#anyURI">http://purl.org/ppeo/PPEO.owl</merge:sourcedFrom><merge:sourceOntology>ppeo</merge:sourceOntology></owl:Class></rdf:RDF>
